MyIO.fst
@@ -1,0 +1,44 @@
+module MyIO
+
+open FStar.All
+
+exception EOF
+assume new type mi_fd_read : Type0
+assume new type mi_fd_write : Type0
+
+assume val mi_print_newline : unit -> ML unit
+assume val mi_print_string : string -> ML unit
+assume val mi_print_uint8 : FStar.UInt8.t -> ML unit
+assume val mi_print_uint8_dec : FStar.UInt8.t -> ML unit
+assume val mi_print_uint32 : FStar.UInt32.t -> ML unit
+assume val mi_print_uint32_dec : FStar.UInt32.t -> ML unit
+assume val mi_print_uint64 : FStar.UInt64.t -> ML unit
+assume val mi_print_uint64_dec : FStar.UInt64.t -> ML unit
+assume val mi_print_any : 'a -> ML unit
+assume val mi_input_line : unit -> ML string
+assume val mi_input_int : unit -> ML int
+assume val mi_input_float : unit -> ML FStar.Float.float
+assume val mi_open_read_file : string -> ML mi_fd_read
+assume val mi_open_write_file : string -> ML mi_fd_write
+assume val mi_close_read_file : mi_fd_read -> ML unit
+assume val mi_close_write_file : mi_fd_write -> ML unit
+assume val mi_read_line : mi_fd_read -> ML string
+assume val mi_write_string : mi_fd_write -> string -> ML unit
+
+assume val mi_readdir : string -> ML (list string)
+assume val mi_file_exists : string -> ML bool
+
+assume val mi_fail: string -> Tot bool
+
+(* assume val *) 
+
+(*
+   An UNSOUND escape hatch for printf-debugging;
+   Although it always returns false, we mark it
+   as returning a bool, so that extraction doesn't
+   erase this call.
+   Note: no guarantees are provided regarding the order
+   of eassume valuation of this function; since it is marked as pure,
+   the compiler may re-order or replicate it.
+*)
+assume val mi_debug_print_string : string -> Tot bool
