StarCombinator.Base.fst
@@ -1,0 +1,107 @@
+module StarCombinator.Base
+
+open StarCombinator.Core
+open FStar.String
+open FStar.Char
+
+module C = StarCombinator.Constants
+module L = FStar.List.Tot.Base
+module M = FStar.Mul
+
+private
+let undefErr p0 p1 = ParserRes None (undefErr p0 p1 "undef")
+
+(** if ch is matched, it output symb  **)
+let satisfy (f: char -> bool) : parser char
+    = fun src pos -> if pos >= FStar.String.length src
+                  then undefErr (if pos = 0 then 0 else pos-1) pos
+                  else (
+                     let current = get src pos in
+                     if f current
+                     then ParserRes (Some (pos+1, current)) noError
+                     else undefErr pos (pos+1)
+                  )
+
+private
+let rec lst_contains (#a:eqtype)  (x: a) (l: list a) = match l with
+  | [] -> false | h::t -> x = h || lst_contains x t
+
+let exact (exactChar: char) : parser char
+    = satisfy (fun c -> c = exactChar) <?> "expected '" ^ string_of_list [exactChar] ^ "'"
+
+let oneOf (possibles: list char): parser char
+    = satisfy (fun c -> lst_contains c possibles) <?> "expected something in the range [" ^ string_of_list possibles ^ "]"
+
+let noneOf (possibles: list char): parser char
+    = satisfy (fun c -> not (lst_contains c possibles)) <?> "expected something out of the range ["^string_of_list possibles^"]"
+
+(** Identity for parsers, in a sense **)
+let match_empty #a (symb: a) : parser a = fun _ pos -> ParserRes (Some (pos, symb)) noError
+
+
+//let space = oneOf C.isSpaceChar
+
+let space = oneOf ('\n'::C.isSpaceChar)
+
+ (* zero one or more spaces *)
+let spaces: parser unit = fp (fun _ -> ()) (many space)
+
+
+let newline = fp (fun _ -> ()) (exact '\n')
+let crlf = fp (fun _ -> ()) (exact '\r' <*> newline)
+
+let endOfLine = newline <|> crlf
+
+let tab =fp (fun _ -> ()) (exact '\t')
+
+let lower = oneOf C.lowerCaseCharList
+let upper = oneOf C.upperCaseCharList
+
+let digit = oneOf C.digitList
+
+let charClass (l:list char {~(l == [])}): parser char = choice (L.map exact l)
+
+let digit_num : parser (n: nat{n <= 9}) = 
+  let convert (c:char): (n: nat{n <= 9}) = match c with
+              | '1' -> 1 | '2' -> 2 | '3' -> 3 | '4' -> 4 | '5' -> 5
+              | '6' -> 6 | '7' -> 7 | '8' -> 8 | '9' -> 9 |  _  -> 0 in
+  fp convert (charClass C.digitList) <?> "expected digit"
+
+let notLetter = (fp (fun _ -> ' ') eof <||> satisfy (fun c -> lst_contains c C.anyCaseCharList)) <?> "expected something different than a letter"
+
+let letter = charClass C.anyCaseCharList <?> "expected letter"
+
+let natural_number : parser nat =
+  let rec convert (c:list (n: nat{n <= 9})): nat = match c with
+    | [] -> 0
+    | hd::tl -> hd + (M.op_Star 10 (convert tl))
+  in
+  fp (fun x -> convert (L.rev x)) (many1 digit_num <<*> notFollowedBy letter) <?> "expected natural number"
+
+let number: parser int = fp (fun ((m, n): (option char*nat)) -> match m with | Some _ -> 1 | None -> n)
+                       (maybe (exact '-') <*> natural_number) <?> "expected number"
+
+
+let alphaNum = charClass (C.digitList @ C.anyCaseCharList) <?> "expected alphanumeric"
+
+let hexDigit = charClass (C.digitList @ list_of_string "ABCDEFabcdef") <?> "expected hex digit"
+
+let exact_string (str:string{str <> ""}): parser string = fp string_of_list (sequence #char (admitP(list_of_string str <> []); L.map exact (list_of_string str))) <?> "expected the exact string \""^str^"\""
+
+let string_satisfy (fchar: char -> bool): parser string = fp string_of_list (many1 (satisfy fchar)) <?> "expected some string maching some predicate"
+
+let word: parser string = (string_satisfy (fun c -> lst_contains c C.anyCaseCharList) <<*> notFollowedBy letter) <?> "expected a word"
+
+let keyword str: parser unit = fp (fun _ -> ()) (spaces <*> exact_string str <*> spaces <<*> notFollowedBy letter) <?> "expected the keyword "^str
+
+let keywords (lstr: list string{lstr<>[]}): parser unit = fp (fun _ -> ()) (sequence #string (admit(); L.map (fun s -> spaces <*>> exact_string s) lstr) <*> spaces) <?> "expected the keywords " ^ (String.concat " " lstr)
+
+let ckwd ch: parser unit = (spaces <<*> exact ch <<*> spaces) <?> "expected char keyword "^(String.string_of_list [ch])
+
+let wrapspace p = spaces <*>> p <<*> spaces
+
+let match_boolean_litterate = ((fp (fun x -> true) (exact_string "true")) <|> (fp (fun x -> false) (exact_string "false"))) <?> "expected false or true"
+
+let between_kwd l r i = between (keyword l) (keyword r) i <?> "expected something of the form \""^l^" ... "^r^"\""
+
+let match_list l r s i = between_kwd l r (sepBy i (keyword s)) <?> "expected a list \""^l^" ... "^s^" ... "^r^"\""
