StarCombinator.Examples.fst
@@ -1,0 +1,49 @@
+module StarCombinator.Examples
+
+open StarCombinator
+open MyIO
+
+open FStar.Mul
+open StarCombinator.Examples.While
+
+let calculator_parser: parser int = 
+    let rec h (_:unit): parser int = (
+      let g = delayMe (admit (); h) in
+          fp (fun (a, b) -> a + b) (number <<*> (keyword "plus" <|> ckwd '+') <*> g)
+      <|> fp (fun (a, b) -> a - b) (number <<*> (keyword "minus"<|> keyword "-") <*> g)
+      <|> fp (fun (a, b) -> a * b) (number <<*> (keywords ["hey";"times"] <|> keyword "*") <*> g)
+      <|> number
+    //and no_lrec () =
+    //       number
+    //  <|> (keyword "Bonjour" <*>> number <<*> keywords ["X";"Y";"Z"])
+    ) in h ()
+
+let calculator source = match (make calculator_parser) source with
+  | Inl intvalue -> "Got some result: " ^ string_of_int intvalue
+  | Inr error -> "Got some error: " ^ error
+
+module All = FStar.All
+module S = FStar.String
+
+let mi_input_lines (): All.ML string =
+  let rec h (): All.ML (list string) =
+    let line = mi_input_line () in
+    if line = "" then [line]
+    else (h ())@[line]
+  in let r = h () in
+  S.concat "\n" r
+
+let x = make lFakeInstr_parser
+
+let main0 () = 
+  let prog = mi_input_line () in
+  mi_print_string (match calculator prog with
+    | r -> r)
+
+let main1 () = 
+  let prog = mi_input_lines () in
+  mi_print_string (match x prog with
+    | Inl _ -> "Succeeds!"
+    | Inr r -> r)
+
+let main = main0 ()
