StarCombinator.Helpers.fst
@@ -1,0 +1,24 @@
+module StarCombinator.Helpers
+
+private
+let prefix = '\x1b'
+
+
+
+let cstHEADER = "\x1b[95m"
+let cstOKBLUE = "\x1b[94m"
+let cstOKGREEN = "\x1b[92m"
+let cstWARNING = "\x1b[93m"
+let cstFAIL = "\x1b[91m"
+let cstENDC = "\x1b[0m"
+let cstBOLD = "\x1b[1m"
+let cstUNDERLINE = "\x1b[4m"
+
+let header str 		= cstHEADER	^ str ^ cstENDC
+let okblue str 		= cstOKBLUE	^ str ^ cstENDC
+let okgreen str 	= cstOKGREEN	^ str ^ cstENDC
+let warning str 	= cstWARNING	^ str ^ cstENDC
+let fail str 		= cstFAIL	^ str ^ cstENDC
+let bold str 		= cstBOLD	^ str ^ cstENDC
+let underline str 	= cstUNDERLINE	^ str ^ cstENDC
+let line str            = str ^ "\n"
