Makefile
@@ -1,0 +1,60 @@
+STAR=/home/FStar/FStar/bin/fstar.exe
+FSTAR_HOME=/home/FStar/FStar/
+CAMLDEP=ocamldep
+
+ifndef FSTAR_HOME
+   $(error "Please define the `FSTAR_HOME` variable before including this makefile.")
+endif
+
+include $(FSTAR_HOME)/ulib/gmake/z3.mk
+include $(FSTAR_HOME)/ulib/gmake/fstar.mk
+
+EXEC = Main.out
+
+ifeq ($(OS),Windows_NT)
+  MSBUILD = $(FSTAR_HOME)/src/msbuild.bat
+else
+  # If can't find msbuild, use xbuild, but throw a warning
+  MSBUILD = $(shell which msbuild || (echo '\n\n\033[0;31mWarning:\033[0m could not find "msbuild", trying (deprecated) "xbuild"\n\n'>&2; which xbuild))
+  # syntax highlightint fix ')
+endif
+
+%.uver: %.fst
+	$(FSTAR) --use_extracted_interfaces true $^
+
+%.fail-uver: %.fst
+	(! $(FSTAR) $^ >/dev/null 2>&1) || (echo "NEGATIVE TEST FAILED ($@)!" ; false)
+
+include $(FSTAR_HOME)/ulib/ml/Makefile.include
+
+
+ROOTS=$(shell echo *.fst)# AbstractDomain.fst CSet.fst CSetPO.fst DefaultValue.fst EnumerableMap.fst ExtInt.fst GaloisConnection.fst Interval.fst Main.fst Misc.fst PartialOrder.fst StaticAnalyser.fst ToString.fst ToyLanguageDef.fst ToyLanguageInterpreter.fst ZeroOrLess.fst
+
+compile:
+	bash compile.sh
+
+gg:
+	mkdir out
+	cp MyIO.ml out/
+	# cp /home/FStar/FStar/ulib/ml/FStar_Char.ml out/
+
+# all: verify-all
+all: gg codegen compile
+
+exec:
+	bash -c "cd out; ./StarCombinator_Examples.native"
+
+x: clean all
+
+test:
+	echo $(OCAMLOPT)
+
+FSTAR_MORESTUFF=--no_extract FStar.BitVector --no_extract MyIO --no_extract FStar.List.Tot --no_extract FStar.List.Tot.Properties --no_extract FStar.Math.Lemmas --no_extract FStar.Math.Lib --no_extract FStar.OrdSet --no_extract FStar.PredicateExtensionality --no_extract FStar.Preorder --no_extract FStar.PropositionalExtensionality --no_extract FStar.Reflection --no_extract FStar.Reflection.Const --no_extract FStar.Reflection.Derived --no_extract FStar.Reflection.Derived.Lemmas --no_extract FStar.Reflection.Formula --no_extract FStar.Seq --no_extract FStar.Seq.Base --no_extract FStar.Seq.Properties --no_extract FStar.StrongExcludedMiddle --no_extract FStar.Tactics --no_extract FStar.Tactics.Derived --no_extract FStar.Tactics.Effect --no_extract FStar.Tactics.Logic --no_extract FStar.Tactics.PatternMatching --no_extract FStar.Tactics.Typeclasses --no_extract FStar.Tactics.Util --no_extract FStar.UInt
+
+# --use_native_int?
+codegen:
+	$(FSTAR) $(FSTAR_DEFAULT_ARGS) $(FSTAR_MORESTUFF) --odir out --codegen OCaml StarCombinator.Examples.fst
+
+clean:
+	rm -f .depend *.checked
+	rm -rf out
