compile.sh
@@ -1,0 +1,10 @@
+cd out
+# echo "let main = print_string \"Number? \"; let strline = read_line () in print_string (Main.getStr strline (Prims.parse_int \"2\"))" > Exec.ml
+# echo "let main = print_string \"Number? \"; let strline = read_line () in print_string (Main.getStr strline (Prims.parse_int strline))" > Exec.ml
+OCAMLPATH=/home/FStar/FStar/bin ocamlbuild -package fstarlib,fstar-tactics-lib,fstar-compiler-lib "StarCombinator_Examples.native"
+# OCAMLPATH=/home/FStar/FStar/bin ocamlbuild -package fstarlib,fstar-tactics-lib,fstar-compiler-lib "Exec.native"
+echo ""
+echo ""
+./StarCombinator_Examples.native
+# ./Exec.native
+echo ""
